improve bvl (and bvi) semantics via an initial empty state
the semantics now does not take a state as argument, but always uses its
own empty state (with the given code and ffi).

to make the observational semantics preservation go through required
proving that the compiler does not introduce duplicate code locations.

compiler/backend/proofs/clos_to_bvlProofScript.sml
@@ -578,6 +578,11 @@ val code_installed_def = Define `
   code_installed aux code =
     EVERY (\(n,num_args,exp). lookup n code = SOME (num_args,exp)) aux`;
 
+val code_installed_fromAList = Q.store_thm("code_installed_fromAList",
+  `ALL_DISTINCT (MAP FST ls) ⇒ code_installed ls (fromAList ls)`,
+  rw[code_installed_def,EVERY_MEM,FORALL_PROD,lookup_fromAList] >>
+  metis_tac[ALOOKUP_ALL_DISTINCT_MEM])
+
 val closure_code_installed_def = Define `
   closure_code_installed code exps_ps (env:closSem$v list) =
     EVERY (\((n,exp),p).
@@ -3702,6 +3707,168 @@ val compile_exps_correct = Q.store_thm("compile_exps_correct",
              `ck + s1.clock − LENGTH args' = ck + (s1.clock − LENGTH args')` by decide_tac >>
              metis_tac []))));
 
+(* more correctness properties *)
+
+val build_aux_thm = prove(
+  ``∀c n aux n7 aux7.
+    build_aux n c aux = (n7,aux7++aux) ⇒
+    (MAP FST aux7) = (REVERSE (GENLIST ($+ n) (LENGTH c)))``,
+  Induct >> simp[build_aux_def] >> rw[] >>
+  qmatch_assum_abbrev_tac`build_aux nn kk auxx = Z` >>
+  qspecl_then[`kk`,`nn`,`auxx`]strip_assume_tac build_aux_acc >>
+  Cases_on`build_aux nn kk auxx`>>UNABBREV_ALL_TAC>>fs[]>> rw[] >>
+  full_simp_tac std_ss [Once (CONS_APPEND)] >>
+  full_simp_tac std_ss [Once (GSYM APPEND_ASSOC)] >> res_tac >>
+  rw[GENLIST,REVERSE_APPEND,REVERSE_GENLIST,PRE_SUB1] >>
+  simp[LIST_EQ_REWRITE])
+
+val lemma =
+  SIMP_RULE(std_ss++LET_ss)[UNCURRY]compile_exps_acc
+
+fun tac (g as (asl,w)) =
+  let
+    fun get tm =
+      let
+        val tm = tm |> strip_forall |> snd |> dest_imp |> fst
+        fun a tm =
+          let
+            val (f,xs) = strip_comb tm
+          in
+            same_const``clos_to_bvl$compile_exps``f andalso
+            length xs = 2
+          end
+      in
+        first a [rhs tm, lhs tm]
+      end
+    val tm = tryfind get asl
+    val args = snd(strip_comb tm)
+  in
+    Cases_on[ANTIQUOTE tm] >>
+    strip_assume_tac(SPECL args lemma) >>
+    rfs[]
+  end g
+
+val compile_exps_code_locs = store_thm("compile_exps_code_locs",
+  ``∀xs aux ys aux2.
+    compile_exps xs aux = (ys,aux2++aux) ⇒
+    MAP FST aux2 = MAP ((+) num_stubs) (REVERSE(code_locs xs))``,
+  ho_match_mp_tac compile_exps_ind >> rpt conj_tac >>
+  TRY (
+    rw[compile_exps_def] >>
+    Cases_on`fns`>>fs[code_locs_def]>-(
+      fs[LET_THM] ) >>
+    Cases_on`t`>>fs[code_locs_def]>-(
+      Cases_on `h` >> fs [] >>
+      rw[LET_THM] >> tac >> tac  >> rw[] >> fs[LET_THM] >> rw[] >> DECIDE_TAC) >>
+    simp[] >> rw[] >>
+    fs[compile_exps_def,LET_THM,UNCURRY] >> rw[] >>
+    qmatch_assum_abbrev_tac`SND (compile_exps [x1] aux1) = aux2 ++ aux` >>
+    qspecl_then[`[x1]`,`aux1`]strip_assume_tac lemma >>
+    Cases_on`compile_exps [x1] aux1`>>fs[Abbr`aux1`] >> rw[] >>
+    qmatch_assum_abbrev_tac`ys++SND(build_aux (loc + num_stubs) aux1 z) = aux2 ++ aux` >>
+    qspecl_then[`aux1`,`loc+num_stubs`,`z`]STRIP_ASSUME_TAC build_aux_acc >>
+    Cases_on`build_aux (loc+num_stubs) aux1 z`>>fs[] >>
+    qspecl_then[`[SND h]`,`aux`]strip_assume_tac lemma >>
+    Cases_on`compile_exps [SND h] aux`>>fs[] >> rw[] >>
+    qspecl_then[`SND h'::MAP SND t'`,`ys'++aux`]strip_assume_tac lemma >>
+    Cases_on`compile_exps (SND h'::MAP SND t') (ys'++aux)`>>fs[] >> rw[] >>
+    fs[Abbr`z`] >> rw[] >> fs[] >>
+    full_simp_tac std_ss [GSYM APPEND_ASSOC]  >>
+    imp_res_tac build_aux_thm >>
+    simp[Abbr`aux1`,ADD1, MAP_REVERSE, LENGTH_MAP2, MAP_GENLIST] >>
+    match_mp_tac (METIS_PROVE [] ``!f x y z. (!a. x a = y a) ⇒ f x z = f y z``) >>
+    simp [combinTheory.o_DEF]) >>
+  simp[compile_exps_def,code_locs_def,UNCURRY] >> rw[] >>
+  rpt tac >> rw[] >> fs[] >> rw[]);
+
+val init_code_ok = Q.store_thm ("init_code_ok",
+  `(!n.
+      n < max_app ⇒ lookup n init_code = SOME (n + 2, generate_generic_app n)) ∧
+   (!m n.
+      m < max_app ∧ n < max_app ⇒
+        lookup (partial_app_fn_location m n) init_code =
+          SOME (m - n + 1, generate_partial_app_closure_fn m n)) ∧
+   (lookup equality_location init_code = SOME equality_code) ∧
+   (lookup block_equality_location init_code = SOME block_equality_code) ∧
+   (lookup ToList_location init_code = SOME ToList_code)`,
+  rw [init_code_def, lookup_fromList, EL_APPEND1, partial_app_fn_location_def]
+  >- decide_tac
+  >- simp[EL_APPEND1]
+  >- (rw [LENGTH_FLAT, MAP_GENLIST, combinTheory.o_DEF, sum_genlist_square] >>
+      rw [DECIDE ``!(x:num) y z n. x + y +n < x + z + a ⇔ y +n < z + a``] >>
+      `max_app * m + n < max_app * max_app` by metis_tac[less_rectangle] >>
+      DECIDE_TAC)
+  >- (`max_app ≤ max_app + max_app * m + n` by decide_tac >>
+      ONCE_REWRITE_TAC[GSYM APPEND_ASSOC] >>
+      simp[EL_APPEND2] >>
+      `n+m*max_app < max_app*max_app` by metis_tac [less_rectangle2] >>
+      `0 < max_app` by rw [max_app_def] >>
+      rw [twod_table] >>
+      asm_simp_tac std_ss [EL_APPEND1,LENGTH_GENLIST] >>
+      rw [EL_GENLIST] >>
+      rw [DIV_MULT, Once ADD_COMM] >>
+      ONCE_REWRITE_TAC [ADD_COMM] >>
+      rw [MOD_MULT])
+  >- (
+    `0 < max_app` by rw [max_app_def] >>
+    rw [twod_table] >>
+    simp[equality_location_def] )
+  >- (
+    `0 < max_app` by rw [max_app_def] >>
+    rw [twod_table] >>
+    simp[EL_APPEND2,equality_location_def] )
+  >- (
+    `0 < max_app` by rw [max_app_def] >>
+    rw [twod_table] >>
+    simp[equality_location_def,block_equality_location_def] )
+  >- (
+    `0 < max_app` by rw [max_app_def] >>
+    rw [twod_table] >>
+    simp[EL_APPEND2,block_equality_location_def,equality_location_def] )
+  >- (
+    `0 < max_app` by rw [max_app_def] >>
+    rw [twod_table] >>
+    simp[ToList_location_def,equality_location_def,block_equality_location_def] )
+  >- (
+    `0 < max_app` by rw [max_app_def] >>
+    rw [twod_table] >>
+    simp[EL_APPEND2,ToList_location_def,block_equality_location_def,equality_location_def] ));
+
+val compile_all_distinct_locs = Q.store_thm("compile_all_distinct_locs",
+  `c.start < num_stubs ∧ compile c e = (c',p) ⇒ ALL_DISTINCT (MAP FST p)`,
+  rw[compile_def] >>
+  fs[compile_def,LET_THM] >>
+  rpt(first_assum(split_applied_pair_tac o lhs o concl)>>fs[]) >>
+  rator_x_assum`compile_exps`mp_tac >>
+  specl_args_of_then``compile_exps``compile_exps_code_locs mp_tac >> rw[] >>
+  simp[ALL_DISTINCT_APPEND] >>
+  `∃z. intro_multi [e] = [z]` by (
+    metis_tac[clos_mtiTheory.intro_multi_sing]) >>
+  `∃z. es = [z]` by (
+    metis_tac
+      [clos_numberTheory.renumber_code_locs_length, SING_HD, SND, LENGTH, ONE]) >>
+  `∃z. es' = [z]` by (
+    metis_tac [clos_removeTheory.remove_SING] ) >>
+  `∃z. es'' = [z]` by (
+    metis_tac
+      [clos_annotateTheory.shift_SING,
+       clos_annotateTheory.annotate_def,
+       clos_freeTheory.free_SING, FST, PAIR,
+       compile_exps_SING] ) >>
+  simp[] >>
+  conj_tac >- (
+    match_mp_tac ALL_DISTINCT_MAP_INJ >>
+    conj_tac >- simp[] >>
+    simp[ALL_DISTINCT_REVERSE] >>
+    simp[clos_annotateProofTheory.annotate_code_locs] >>
+    fs[clos_numberTheory.renumber_code_locs_def,LET_THM] >>
+    first_assum(split_applied_pair_tac o lhs o concl) >> fs[] >>
+    metis_tac[clos_removeProofTheory.remove_distinct_locs,FST,SND,
+              clos_numberProofTheory.renumber_code_locs_distinct] ) >>
+  simp[MAP_MAP_o,o_DEF,MEM_MAP,PULL_EXISTS] );
+
+(* composed compiler correctness *)
+
 val full_state_rel_def = Define`
   full_state_rel s1 s2 ⇔
     ∀k. ∃sa sb sc sd f.
@@ -3887,12 +4054,11 @@ val compile_evaluate = Q.store_thm("compile_evaluate",
 
 val compile_semantics = Q.store_thm("compile_semantics",
   `¬contains_App_SOME [e] ∧ every_Fn_vs_NONE [e] ∧
-   compile c e = (c',p)  ∧
-   full_state_rel (s:'ffi closSem$state) s1 ∧
-   code_installed p s1.code ∧
+   compile c e = (c',p) ∧ c.start < num_stubs ∧
+   full_state_rel (s:'ffi closSem$state) (initial_state s.ffi (fromAList p) s.clock) ∧
    semantics [] s [e] ≠ Fail
    ⇒
-   semantics s1 c'.start =
+   semantics s.ffi (fromAList p) c'.start =
    semantics [] s [e]`,
   simp[GSYM AND_IMP_INTRO] >> ntac 5 strip_tac >>
   simp[closSemTheory.semantics_def] >>
@@ -3906,6 +4072,7 @@ val compile_semantics = Q.store_thm("compile_semantics",
     imp_res_tac full_state_rel_with_clock >>
     pop_assum(qspec_then`k`strip_assume_tac) >>
     rpt(disch_then(fn th => first_assum(mp_tac o MATCH_MP th))) >> simp[] >>
+    discharge_hyps >- metis_tac[code_installed_fromAList,compile_all_distinct_locs] >>
     strip_tac >>
     simp[bvlSemTheory.semantics_def] >>
     `r1 ≠ Rerr (Rabort Rtimeout_error) ∧
@@ -3951,6 +4118,7 @@ val compile_semantics = Q.store_thm("compile_semantics",
     imp_res_tac full_state_rel_with_clock >>
     pop_assum(qspec_then`k`strip_assume_tac) >>
     rpt(first_assum(match_exists_tac o concl)>>simp[]) >>
+    conj_tac >- metis_tac[code_installed_fromAList,compile_all_distinct_locs] >>
     spose_not_then strip_assume_tac >>
     qmatch_assum_abbrev_tac`FST q = _` >>
     Cases_on`q`>>fs[markerTheory.Abbrev_def] >>
@@ -3973,6 +4141,7 @@ val compile_semantics = Q.store_thm("compile_semantics",
     imp_res_tac full_state_rel_with_clock >>
     pop_assum(qspec_then`k`strip_assume_tac) >>
     rpt(first_assum(match_exists_tac o concl)>>simp[]) >>
+    conj_tac >- metis_tac[code_installed_fromAList,compile_all_distinct_locs] >>
     spose_not_then strip_assume_tac >>
     first_x_assum(qspec_then`k`strip_assume_tac) >> rfs[] >>
     imp_res_tac evaluate_add_clock >>
@@ -3993,7 +4162,7 @@ val compile_semantics = Q.store_thm("compile_semantics",
     qx_genl_tac[`k1`,`k2`] >>
     qspecl_then[`k1`,`k2`]mp_tac LESS_EQ_CASES >>
     metis_tac[
-      LESS_EQ_EXISTS,
+      LESS_EQ_EXISTS, initial_state_with_simp,
       closPropsTheory.evaluate_add_to_clock_io_events_mono
         |> CONJUNCT1 |> CONV_RULE(RESORT_FORALL_CONV List.rev)
         |> Q.SPEC`s with clock := k` |> SIMP_RULE (srw_ss())[],
@@ -4013,8 +4182,12 @@ val compile_semantics = Q.store_thm("compile_semantics",
   (compile_evaluate
    |> Q.GEN`s` |> Q.SPEC`s with clock := k`
    |> GEN_ALL |> SIMP_RULE(srw_ss()++QUANT_INST_ss[pair_default_qp])[]
-   |> Q.SPECL[`s1 with clock := k`,`s`,`k`,`e`,`c`]
-   |> mp_tac) >> simp[full_state_rel_with_clock] >>
+   |> Q.SPECL[`initial_state (s:'ffi closSem$state).ffi (fromAList p) k`,`s`,`k`,`e`,`c`]
+   |> mp_tac) >>
+  (discharge_hyps >- (
+    simp[] >>
+    metis_tac[full_state_rel_with_clock,initial_state_with_simp,
+              compile_all_distinct_locs, code_installed_fromAList] )) >>
   rw[] >>
   qmatch_assum_abbrev_tac`full_result_rel p1 p2` >>
   Cases_on`p1`>>Cases_on`p2`>>fs[markerTheory.Abbrev_def] >>
@@ -4025,12 +4198,13 @@ val compile_semantics = Q.store_thm("compile_semantics",
               semanticPrimitivesTheory.result_11,
               semanticPrimitivesTheory.error_result_11,
               semanticPrimitivesTheory.abort_distinct])
-  >- ( qexists_tac`ck+k` >> fs[] ) >>
+  >- ( qexists_tac`k+ck` >> fs[] ) >>
   qexists_tac`k` >> fs[] >>
   qmatch_assum_abbrev_tac`n < (LENGTH (_ ffi))` >>
   `ffi.io_events ≼ b2.ffi.io_events` by (
     qunabbrev_tac`ffi` >>
     metis_tac[
+      initial_state_with_simp,
       bvlPropsTheory.evaluate_add_to_clock_io_events_mono
         |> CONV_RULE(RESORT_FORALL_CONV(sort_vars["s"]))
         |> Q.SPEC`s with clock := k`
@@ -4038,180 +4212,9 @@ val compile_semantics = Q.store_thm("compile_semantics",
       SND,ADD_SYM]) >>
   fs[IS_PREFIX_APPEND] >> simp[EL_APPEND1]);
 
-(* more correctness properties *)
-
-val init_code_ok = Q.store_thm ("init_code_ok",
-  `(!n.
-      n < max_app ⇒ lookup n init_code = SOME (n + 2, generate_generic_app n)) ∧
-   (!m n.
-      m < max_app ∧ n < max_app ⇒
-        lookup (partial_app_fn_location m n) init_code =
-          SOME (m - n + 1, generate_partial_app_closure_fn m n)) ∧
-   (lookup equality_location init_code = SOME equality_code) ∧
-   (lookup block_equality_location init_code = SOME block_equality_code) ∧
-   (lookup ToList_location init_code = SOME ToList_code)`,
-  rw [init_code_def, lookup_fromList, EL_APPEND1, partial_app_fn_location_def]
-  >- decide_tac
-  >- simp[EL_APPEND1]
-  >- (rw [LENGTH_FLAT, MAP_GENLIST, combinTheory.o_DEF, sum_genlist_square] >>
-      rw [DECIDE ``!(x:num) y z n. x + y +n < x + z + a ⇔ y +n < z + a``] >>
-      `max_app * m + n < max_app * max_app` by metis_tac[less_rectangle] >>
-      DECIDE_TAC)
-  >- (`max_app ≤ max_app + max_app * m + n` by decide_tac >>
-      ONCE_REWRITE_TAC[GSYM APPEND_ASSOC] >>
-      simp[EL_APPEND2] >>
-      `n+m*max_app < max_app*max_app` by metis_tac [less_rectangle2] >>
-      `0 < max_app` by rw [max_app_def] >>
-      rw [twod_table] >>
-      asm_simp_tac std_ss [EL_APPEND1,LENGTH_GENLIST] >>
-      rw [EL_GENLIST] >>
-      rw [DIV_MULT, Once ADD_COMM] >>
-      ONCE_REWRITE_TAC [ADD_COMM] >>
-      rw [MOD_MULT])
-  >- (
-    `0 < max_app` by rw [max_app_def] >>
-    rw [twod_table] >>
-    simp[equality_location_def] )
-  >- (
-    `0 < max_app` by rw [max_app_def] >>
-    rw [twod_table] >>
-    simp[EL_APPEND2,equality_location_def] )
-  >- (
-    `0 < max_app` by rw [max_app_def] >>
-    rw [twod_table] >>
-    simp[equality_location_def,block_equality_location_def] )
-  >- (
-    `0 < max_app` by rw [max_app_def] >>
-    rw [twod_table] >>
-    simp[EL_APPEND2,block_equality_location_def,equality_location_def] )
-  >- (
-    `0 < max_app` by rw [max_app_def] >>
-    rw [twod_table] >>
-    simp[ToList_location_def,equality_location_def,block_equality_location_def] )
-  >- (
-    `0 < max_app` by rw [max_app_def] >>
-    rw [twod_table] >>
-    simp[EL_APPEND2,ToList_location_def,block_equality_location_def,equality_location_def] ));
-
 (* TODO: cleanup, move, or delete things below *)
 
 (*
-
-val build_aux_thm = prove(
-  ``∀c n aux n7 aux7.
-    build_aux n c aux = (n7,aux7++aux) ⇒
-    (MAP FST aux7) = (REVERSE (GENLIST ($+ n) (LENGTH c)))``,
-  Induct >> simp[build_aux_def] >> rw[] >>
-  qmatch_assum_abbrev_tac`build_aux nn kk auxx = Z` >>
-  qspecl_then[`kk`,`nn`,`auxx`]strip_assume_tac build_aux_acc >>
-  Cases_on`build_aux nn kk auxx`>>UNABBREV_ALL_TAC>>fs[]>> rw[] >>
-  full_simp_tac std_ss [Once (CONS_APPEND)] >>
-  full_simp_tac std_ss [Once (GSYM APPEND_ASSOC)] >> res_tac >>
-  rw[GENLIST,REVERSE_APPEND,REVERSE_GENLIST,PRE_SUB1] >>
-  simp[LIST_EQ_REWRITE])
-
-val lemma =
-  SIMP_RULE(std_ss++LET_ss)[UNCURRY]compile_exps_acc
-
-fun tac (g as (asl,w)) =
-  let
-    fun get tm =
-      let
-        val tm = tm |> strip_forall |> snd |> dest_imp |> fst
-        fun a tm =
-          let
-            val (f,xs) = strip_comb tm
-          in
-            same_const``compile_exps``f andalso
-            length xs = 2
-          end
-      in
-        first a [rhs tm, lhs tm]
-      end
-    val tm = tryfind get asl
-    val args = snd(strip_comb tm)
-  in
-    Cases_on[ANTIQUOTE tm] >>
-    strip_assume_tac(SPECL args lemma) >>
-    rfs[]
-  end g
-
-val compile_exps_code_locs = store_thm("compile_exps_code_locs",
-  ``∀xs aux ys aux2.
-    compile_exps xs aux = (ys,aux2++aux) ⇒
-    MAP FST aux2 = MAP ((+) num_stubs) (REVERSE(code_locs xs))``,
-  ho_match_mp_tac compile_exps_ind >> rpt conj_tac >>
-  TRY (
-    rw[compile_exps_def] >>
-    Cases_on`fns`>>fs[code_locs_def]>-(
-      fs[LET_THM] ) >>
-    Cases_on`t`>>fs[code_locs_def]>-(
-      Cases_on `h` >> fs [] >>
-      rw[LET_THM] >> tac >> tac  >> rw[] >> fs[LET_THM] >> rw[] >> DECIDE_TAC) >>
-    simp[] >> rw[] >>
-    fs[compile_exps_def,LET_THM,UNCURRY] >> rw[] >>
-    qmatch_assum_abbrev_tac`SND (compile_exps [x1] aux1) = aux2 ++ aux` >>
-    qspecl_then[`[x1]`,`aux1`]strip_assume_tac lemma >>
-    Cases_on`compile_exps [x1] aux1`>>fs[Abbr`aux1`] >> rw[] >>
-    qmatch_assum_abbrev_tac`ys++SND(build_aux (loc + num_stubs) aux1 z) = aux2 ++ aux` >>
-    qspecl_then[`aux1`,`loc+num_stubs`,`z`]STRIP_ASSUME_TAC build_aux_acc >>
-    Cases_on`build_aux (loc+num_stubs) aux1 z`>>fs[] >>
-    qspecl_then[`[SND h]`,`aux`]strip_assume_tac lemma >>
-    Cases_on`compile_exps [SND h] aux`>>fs[] >> rw[] >>
-    qspecl_then[`SND h'::MAP SND t'`,`ys'++aux`]strip_assume_tac lemma >>
-    Cases_on`compile_exps (SND h'::MAP SND t') (ys'++aux)`>>fs[] >> rw[] >>
-    fs[Abbr`z`] >> rw[] >> fs[] >>
-    full_simp_tac std_ss [GSYM APPEND_ASSOC]  >>
-    imp_res_tac build_aux_thm >>
-    simp[Abbr`aux1`,ADD1, MAP_REVERSE, LENGTH_MAP2, MAP_GENLIST] >>
-    match_mp_tac (METIS_PROVE [] ``!f x y z. (!a. x a = y a) ⇒ f x z = f y z``) >>
-    simp [combinTheory.o_DEF]) >>
-  simp[compile_exps_def,code_locs_def,UNCURRY] >> rw[] >>
-  rpt tac >> rw[] >> fs[] >> rw[]);
-
-val code_locs_def = tDefine "code_locs" `
-  (code_locs [] = []) /\
-  (code_locs (x::y::xs) =
-     let c1 = code_locs [x] in
-     let c2 = code_locs (y::xs) in
-       c1 ++ c2) /\
-  (code_locs [Var v] = []) /\
-  (code_locs [If x1 x2 x3] =
-     let c1 = code_locs [x1] in
-     let c2 = code_locs [x2] in
-     let c3 = code_locs [x3] in
-       c1 ++ c2 ++ c3) /\
-  (code_locs [Let xs x2] =
-     let c1 = code_locs xs in
-     let c2 = code_locs [x2] in
-       c1 ++ c2) /\
-  (code_locs [Raise x1] =
-     code_locs [x1]) /\
-  (code_locs [Handle x1 x2] =
-     let c1 = code_locs [x1] in
-     let c2 = code_locs [x2] in
-       c1 ++ c2) /\
-  (code_locs [Tick x1] =
-     code_locs [x1]) /\
-  (code_locs [Op op xs] =
-     case op of
-       Label loc => code_locs xs ++ [loc]
-     | _ => code_locs xs) /\
-  (code_locs [Call ticks dest xs] =
-     case dest of NONE => code_locs xs
-                | SOME loc => loc::code_locs xs)`
- (WF_REL_TAC `measure (bvl_exp1_size)`
-  \\ REPEAT STRIP_TAC \\ DECIDE_TAC);
-
-val code_locs_cons = store_thm("code_locs_cons",
-  ``∀x xs. code_locs (x::xs) = code_locs [x] ++ code_locs xs``,
-  gen_tac >> Cases >> simp[code_locs_def])
-
-val code_locs_append = store_thm("code_locs_append",
-  ``∀l1 l2. clos_to_bvl$code_locs (l1 ++ l2) = code_locs l1 ++ code_locs l2``,
-  Induct >> simp[code_locs_def] >>
-  simp[Once code_locs_cons] >>
-  simp[Once code_locs_cons,SimpRHS])
 
 val code_locs_MAP_Var = store_thm("code_locs_MAP_Var",
   ``code_locs (MAP Var xs) = []``,
